Compilable versions of the LinearMaybe and LinearSequence specs

lib/Lang/LinearExtern.h
@@ -1,0 +1,147 @@
+#include "DafnyRuntime.h"
+
+#include <vector>
+
+namespace LinearMaybe {
+////////////////////////////////////////////////////////////
+//
+//   Maybe
+//
+////////////////////////////////////////////////////////////
+
+template <typename A>
+struct maybe {
+  A a;
+};
+
+template <typename A>
+A peek(maybe<A> m) { return m.a; }
+
+template <typename A>
+A unwrap(maybe<A> m) { return m.a; }
+
+template <typename A>
+maybe<A> give(A a) { 
+  struct maybe<A> m;
+  m.a = a;
+  return m;
+}
+
+template <typename A>
+//maybe<A> empty() { return maybe(get_default<A>::call()); }
+maybe<A> empty() { 
+  struct maybe<A> m;
+  return m;  // REVIEW: Safe, b/c !has ?
+}    
+
+template <typename A>
+Tuple0 discard(maybe<A> m) { (void)m; Tuple0 ret; return ret; } 
+
+}
+
+template<typename A>
+struct get_default<LinearMaybe::maybe<A>> {
+  static LinearMaybe::maybe<A> call() { 
+    struct LinearMaybe::maybe<A> m;
+    m.a = get_default<A>::call();
+    return m; 
+  }
+};
+
+namespace LinearExtern {
+
+////////////////////////////////////////////////////////////
+//
+//   Ints (for testing purposes)
+//
+////////////////////////////////////////////////////////////
+
+uint64 MakeLinearInt(uint64 u) { return u; }
+void DiscardLinearInt(uint64 u) { (void) u; }
+
+////////////////////////////////////////////////////////////
+//
+//   Linear sequences
+//
+////////////////////////////////////////////////////////////
+
+template <typename A>
+using linear_seq = std::vector<A>;
+
+template <typename A>
+A seq_get(linear_seq<A> s, uint64 i) {
+  return s[i];
+}
+
+template <typename A>
+linear_seq<A> seq_set(linear_seq<A> s, uint64 i, A a) {
+  s[i] = a;
+  return s;
+}
+
+template <typename A>
+uint64 seq_length(linear_seq<A> s) {
+  return s.size();
+}
+
+template <typename A>
+linear_seq<A> seq_alloc(uint64 length) {
+  linear_seq<A> ret;
+  ret.assign(length, get_default<A>::call());
+  return ret;
+}
+
+template <typename A>
+Tuple0 seq_free(linear_seq<A> s) {
+  s.clear();
+  Tuple0 ret;
+  return ret;
+}
+
+template <typename A>
+DafnySequence<A> seq_unleash(linear_seq<A> s) {
+  DafnySequence<A> ret(s);  // Copies contents of s into ret
+  seq_free(s);
+  return ret;
+}
+
+////////////////////////////////////////////////////////////
+//
+//   lseqs
+//
+////////////////////////////////////////////////////////////
+template <typename A>
+using lseq = std::vector<LinearMaybe::maybe<A>>;
+
+template <typename A>
+uint64 lseq_length_raw(lseq<A> s) {
+  return s.size();
+}
+
+template <typename A>
+lseq<A> lseq_alloc_raw(uint64 length) {
+  lseq<A> ret;
+  ret.assign(length, get_default<LinearMaybe::maybe<A>>::call());
+  return ret;
+}
+
+template <typename A>
+Tuple0 lseq_free_raw(lseq<A> s) {
+  s.clear();
+  Tuple0 ret;
+  return ret;
+}
+
+template <typename A>
+Tuple2<lseq<A>, LinearMaybe::maybe<A>> lseq_swap_raw_fun(lseq<A> s1, uint64 i, LinearMaybe::maybe<A> a1) {
+  Tuple2 ret(s1, s1[i]);
+  s1[i] = a1;
+  return ret;
+}
+
+template <typename A>
+LinearMaybe::maybe<A> lseq_share_raw(lseq<A> s, uint64 i) {
+  return s[i];
+}
+
+}
