lib/Lang/LinearMaybe.s.dfy
@@ -1,31 +1,29 @@
 
-module LinearMaybe {
+module {:extern "LinearMaybe"} LinearMaybe {
+  type {:extern "predefined"} maybe(!new)<A>
 
-  type maybe(!new)<A>
-
-  // andrea: I don't like has as a name, I can't quite say it right
-  predicate has<A>(m:maybe<A>)
+  predicate {:axiom} has<A>(m:maybe<A>)
 
   // return value in m if has(m), return default ghost A value otherwise
-  function read<A>(m:maybe<A>):A
+  function {:axiom} read<A>(m:maybe<A>):A
 
-  function method peek<A>(shared m:maybe<A>):(shared a:A)
+  function method {:extern "LinearMaybe", "peek"} peek<A>(shared m:maybe<A>):(shared a:A)
     requires has(m)
     ensures a == read(m)
 
-  function method unwrap<A>(linear m:maybe<A>):(linear a:A)
+  function method {:extern "LinearMaybe", "unwrap"} unwrap<A>(linear m:maybe<A>):(linear a:A)
     requires has(m)
     ensures a == read(m)
 
-  function method give<A>(linear a:A):(linear m:maybe<A>)
+  function method {:extern "LinearMaybe", "give"} give<A>(linear a:A):(linear m:maybe<A>)
     ensures has(m)
     ensures read(m) == a
     ensures forall x:maybe<A> {:trigger give(read(x))} | has(x) && a == read(x) :: m == x
 
-  function method empty<A>():(linear m:maybe<A>)
+  function method {:extern "LinearMaybe", "empty"} empty<A>():(linear m:maybe<A>)
     ensures !has(m)
 
-  function method discard<A>(linear m:maybe<A>):()
+  function method {:extern "LinearMaybe", "discard"} discard<A>(linear m:maybe<A>):()
     requires !has(m)
 
 } // module
