lib/Lang/LinearSequence.s.dfy
@@ -1,67 +1,63 @@
 include "NativeTypes.s.dfy"
 include "LinearMaybe.s.dfy"
 
-module LinearSequence_s {
+module {:extern "LinearExtern"} LinearSequence_s {
   import opened NativeTypes
   import opened LinearMaybe
 
-  function method seq_get<A>(shared s:seq<A>, i:uint64):(a:A)
+  function method {:extern "LinearExtern", "seq_get"} seq_get<A>(shared s:seq<A>, i:uint64):(a:A)
       requires i as int < |s|
       ensures a == s[i]
 
-  function method seq_set<A>(linear s1:seq<A>, i:uint64, a:A):(linear s2:seq<A>) // can be implemented as in-place update
+  function method {:extern "LinearExtern", "seq_set"} seq_set<A>(linear s1:seq<A>, i:uint64, a:A):(linear s2:seq<A>) // can be implemented as in-place update
       requires i as nat < |s1|
       ensures s2 == s1[i as nat := a]
 
-  function method seq_length<A>(shared s:seq<A>):(n:nat)
-      ensures n == |s|
+  function method {:extern "LinearExtern", "seq_length"} seq_length<A>(shared s:seq<A>):(n:uint64)
+      ensures n as int == |s|
 
-  function method seq_alloc<A>(length:uint64):(linear s:seq<A>)
+  function method {:extern "LinearExtern", "seq_alloc"} seq_alloc<A>(length:uint64):(linear s:seq<A>)
       ensures |s| == length as int
 
-  function method seq_free<A>(linear s:seq<A>):()
+  function method {:extern "LinearExtern", "seq_free"} seq_free<A>(linear s:seq<A>):()
 
-  function method seq_unleash<A>(linear s1:seq<A>):(s2:seq<A>)
+  function method {:extern "LinearExtern", "seq_unleash"} seq_unleash<A>(linear s1:seq<A>):(s2:seq<A>)
       ensures s1 == s2
 
-  type lseq<A>
 
-  function lseqs_raw<A>(l:lseq<A>):(s:seq<maybe<A>>) // contents of an lseq, as ghost seq
+  type {:extern "predefined"} lseq<A>
+
+  function {:axiom} lseqs_raw<A>(l:lseq<A>):(s:seq<maybe<A>>) // contents of an lseq, as ghost seq
     ensures rank_is_less_than(s, l)
 
-  lemma axiom_lseqs_rank<A>(l:lseq<A>, s:seq<A>)
+  lemma {:axiom} axiom_lseqs_rank<A>(l:lseq<A>, s:seq<A>)
     requires |lseqs_raw(l)| == |s|
     requires forall i :: 0 <= i < |s| ==> s[i] == read(lseqs_raw(l)[i])
     ensures rank_is_less_than(s, l)
 
   // it's okay to synthesize all the lseqs you want if they're ghosty
-  function imagine_lseq_raw<A>(s:seq<A>):(l:lseq<A>)
-    ensures lseq_length_raw(l) == |s|
+  function {:axiom} imagine_lseq_raw<A>(s:seq<A>):(l:lseq<A>)
+    requires |s| < 0x1_0000_0000_0000_0000
+    ensures lseq_length_raw(l) as int == |s|
     ensures forall i :: 0 <= i < |s| ==> s[i] == read(lseqs_raw(l)[i])
 
-  function method lseq_length_raw<A>(shared s:lseq<A>):(n:nat)
-      ensures n == |lseqs_raw(s)|
+  function method {:extern "LinearExtern", "lseq_length_raw"} lseq_length_raw<A>(shared s:lseq<A>):(n:uint64)
+      ensures n as int == |lseqs_raw(s)|
 
-  function method lseq_alloc_raw<A>(length:uint64):(linear s:lseq<A>)
+  function method {:extern "LinearExtern", "lseq_alloc_raw"} lseq_alloc_raw<A>(length:uint64):(linear s:lseq<A>)
       ensures |lseqs_raw(s)| == length as nat
       ensures forall i:nat | i < length as nat :: !has(lseqs_raw(s)[i])
 
-  function method lseq_free_raw<A>(linear s:lseq<A>):()
+  function method {:extern "LinearExtern", "lseq_free_raw"} lseq_free_raw<A>(linear s:lseq<A>):()
       requires forall i:nat | i < |lseqs_raw(s)| :: !has(lseqs_raw(s)[i])
 
   // can be implemented as in-place swap
-  method lseq_swap_raw<A>(linear s1:lseq<A>, i:uint64, linear a1:maybe<A>) returns(linear s2:lseq<A>, linear a2:maybe<A>)
-      requires i as nat < |lseqs_raw(s1)|
-      ensures a2 == lseqs_raw(s1)[i as nat]
-      ensures lseqs_raw(s2) == lseqs_raw(s1)[i as nat := a1]
-
-  // can be implemented as in-place swap
-  function method lseq_swap_raw_fun<A>(linear s1:lseq<A>, i:nat, linear a1:maybe<A>):(linear p:(linear lseq<A>, linear maybe<A>))
-      requires i < |lseqs_raw(s1)|
+  function method {:extern "LinearExtern", "lseq_swap_raw_fun"} lseq_swap_raw_fun<A>(linear s1:lseq<A>, i:uint64, linear a1:maybe<A>):(linear p:(linear lseq<A>, linear maybe<A>))
+      requires i as int < |lseqs_raw(s1)|
       ensures p.1 == lseqs_raw(s1)[i]
-      ensures lseqs_raw(p.0) == lseqs_raw(s1)[i := a1]
+      ensures lseqs_raw(p.0) == lseqs_raw(s1)[i as int := a1]
 
-  function method lseq_share_raw<A>(shared s:lseq<A>, i:uint64):(shared a:maybe<A>)
+  function method {:extern "LinearExtern", "lseq_share_raw"} lseq_share_raw<A>(shared s:lseq<A>, i:uint64):(shared a:maybe<A>)
       requires i as int < |lseqs_raw(s)|
       ensures a == lseqs_raw(s)[i]
 
